theories/equivalence/StringUtils.v
@@ -23,7 +23,9 @@ Fixpoint label_in_instr p_str (lbl : label)  :=
   match p_str with
   | [] => false
   | StringLang.Instr opt_lbl _ :: t => match opt_lbl with 
-                                       | Some lbl' => eqb_lbl lbl lbl'
-                                       | None => false
+                                       | Some lbl' => if eqb_lbl lbl lbl'
+                                                      then true
+                                                      else label_in_instr t lbl
+                                       | None => label_in_instr t lbl
                                        end
   end.
